verify NewProph

src/program_proof/mvcc/proph_proof.v
@@ -1,3 +1,4 @@
+From Perennial.goose_lang.lib Require Import proph.proph.
 From Perennial.program_proof.mvcc Require Import mvcc_prelude mvcc_ghost mvcc_action.
 From Perennial.program_proof.mvcc Require Import wrbuf_proof.
 From Perennial.goose_lang.trusted.github_com.mit_pdos.go_mvcc Require Import trusted_proph.
@@ -6,19 +7,55 @@ Section proph.
 Context `{!heapGS Σ}.
 
 (* FIXME: define and prove these. *)
+Local Definition decode_ev_read (v : val) : option action :=
+  match v with
+  | (#(LitInt tid), #(LitInt key))%V => Some (EvRead (int.nat tid) key)
+  | _ => None
+  end.
+Local Definition decode_ev_abort (v : val) : option action :=
+  match v with
+  | #(LitInt tid) => Some (EvAbort (int.nat tid))
+  | _ => None
+  end.
+Local Definition decode_ev_commit (v : val) : option action :=
+  (* FIXME *) None.
 
-Definition mvcc_proph (γ : mvcc_names) (p : proph_id) (acs : list action) : iProp Σ.
-Admitted.
+Local Definition decode_action (v : val) : option action :=
+  match v with
+  | (#(LitInt id), data)%V =>
+      if decide (id = EvReadId) then
+        decode_ev_read data
+      else if decide (id = EvAbortId) then
+        decode_ev_abort data
+      else if decide (id = EvCommitId) then
+        decode_ev_commit data
+      else
+        None
+  | _ => None
+  end.
+Local Fixpoint decode_actions (pvs : list val) : list action :=
+  match pvs with
+  | [] => []
+  | v :: pvs => option_list (decode_action v) ++ decode_actions pvs
+  end.
+
+Definition mvcc_proph (γ : mvcc_names) (p : proph_id) (acs : list action) : iProp Σ :=
+  ∃ (pvs : list val), ⌜decode_actions pvs = acs⌝ ∗ proph p pvs.
 
 Global Instance mvcc_proph_timeless γ p acs :
   Timeless (mvcc_proph γ p acs).
-Admitted.
+Proof. apply _. Qed.
 
 Lemma wp_NewProphActions γ :
   {{{ True }}}
     NewProph #()
   {{{ (p : proph_id) acs, RET #p; mvcc_proph γ p acs }}}.
-Admitted.
+Proof.
+  iIntros (Φ) "_ HΦ". wp_lam.
+  wp_apply wp_new_proph. iIntros (pvs p) "Hp".
+  iApply ("HΦ" $! p (decode_actions pvs)).
+  iExists _. by iFrame.
+Qed.
 
 Lemma wp_ResolveRead γ p (tid key : u64) (ts : nat) :
   ⊢ {{{ ⌜int.nat tid = ts⌝ }}}
@@ -45,3 +82,5 @@ Lemma wp_ResolveCommit γ p (tid : u64) (ts : nat) (wrbuf : loc) (m : dbmap) :
 Admitted.
 
 End proph.
+
+Global Typeclasses Opaque mvcc_proph.
